Add generic session map to factorize code

fstar/MLS.TreeSync.Symbolic.API.GroupManager.fst
@@ -6,166 +6,46 @@ open ComparseGlue
 open GlobalRuntimeLib
 open LabeledRuntimeAPI
 open MLS.Symbolic
-open MLS.Symbolic.Session
-open MLS.Symbolic.TypedSession
+open MLS.Symbolic.MapSession
 
-type group_manager_state_elem_ (bytes:Type0) {|bytes_like bytes|} = {
-  group_id: mls_bytes bytes;
+(*** Group manager types & invariants ***)
+
+type group_manager_value (bytes:Type0) {|bytes_like bytes|} = {
   [@@@ with_parser #bytes ps_nat]
   si_public: nat;
   [@@@ with_parser #bytes ps_nat]
   si_private: nat;
 }
 
-%splice [ps_group_manager_state_elem_] (gen_parser (`group_manager_state_elem_))
-%splice [ps_group_manager_state_elem__is_valid] (gen_is_valid_lemma (`group_manager_state_elem_))
+%splice [ps_group_manager_value] (gen_parser (`group_manager_value))
+%splice [ps_group_manager_value_is_valid] (gen_is_valid_lemma (`group_manager_value))
 
-type group_manager_state_ (bytes:Type0) {|bytes_like bytes|} = {
-  // List of (group_id & public session number & private session number)
-  [@@@ with_parser #bytes (ps_list ps_group_manager_state_elem_)]
-  group_sessions: list (group_manager_state_elem_ bytes);
+val group_manager_types: map_types dy_bytes
+let group_manager_types = {
+  key = mls_bytes dy_bytes;
+  ps_key = ps_mls_bytes;
+  value = group_manager_value dy_bytes;
+  ps_value = ps_group_manager_value;
 }
 
-%splice [ps_group_manager_state_] (gen_parser (`group_manager_state_))
-%splice [ps_group_manager_state__is_valid] (gen_is_valid_lemma (`group_manager_state_))
-
-type group_manager_state_elem = group_manager_state_elem_ dy_bytes
-type group_manager_state = group_manager_state_ dy_bytes
-
-instance parseable_serializeable_group_manager_state: parseable_serializeable dy_bytes group_manager_state = mk_parseable_serializeable ps_group_manager_state_
+val group_manager_pred: map_predicate group_manager_types
+let group_manager_pred = {
+  pred = (fun gu time (group_id:group_manager_types.key) value ->
+    is_publishable gu time group_id
+  );
+  pred_later = (fun gu time0 time1 key value -> ());
+  pred_is_msg = (fun gu time key value -> ());
+}
 
 val group_manager_label: string
 let group_manager_label = "MLS.TreeSync.GroupManager"
 
-val group_manager_state_elem_invariant: global_usage -> timestamp -> group_manager_state_elem -> prop
-let group_manager_state_elem_invariant gu time x =
-  is_publishable gu time x.group_id
-
-val group_manager_state_invariant: global_usage -> timestamp -> group_manager_state -> prop
-let group_manager_state_invariant gu time st =
-  for_allP (group_manager_state_elem_invariant gu time) st.group_sessions
-
-val group_manager_state_invariant_eq: gu:global_usage -> time:timestamp -> st:group_manager_state -> Lemma
-  (group_manager_state_invariant gu time st <==> (forall x. List.Tot.memP x st.group_sessions ==> group_manager_state_elem_invariant gu time x))
-let group_manager_state_invariant_eq gu time st =
-  for_allP_eq (group_manager_state_elem_invariant gu time) st.group_sessions
-
-val bare_group_manager_invariant: bare_typed_session_pred group_manager_state
-let bare_group_manager_invariant gu p time si vi st =
-  group_manager_state_invariant gu time st
-
-val group_manager_invariant: session_pred
-let group_manager_invariant =
-  typed_session_pred_to_session_pred (
-    mk_typed_session_pred bare_group_manager_invariant
-      (fun gu p time0 time1 si vi st ->
-        group_manager_state_invariant_eq gu time0 st;
-        group_manager_state_invariant_eq gu time1 st
-      )
-      (fun gu p time si vi st ->
-        let pre = is_msg gu (readers [psv_id p si vi]) time in
-        group_manager_state_invariant_eq gu time st;
-        for_allP_eq (ps_group_manager_state_elem_.is_valid pre) st.group_sessions
-      )
-  )
-
 val has_group_manager_invariant: preds -> prop
 let has_group_manager_invariant pr =
-  has_session_pred pr group_manager_label group_manager_invariant
+  has_map_session_invariant group_manager_types group_manager_pred group_manager_label pr
 
-(*** AS cache API ***)
+(*** Group manager API ***)
 
-#push-options "--fuel 1"
-val initialize_group_manager:
-  pr:preds -> p:principal -> LCrypto nat pr
-  (requires fun t0 -> has_group_manager_invariant pr)
-  (ensures fun t0 r t1 -> trace_len t1 == trace_len t0 + 1)
-let initialize_group_manager pr p =
-  let time = global_timestamp () in
-  let si = new_session_number pr p in
-  let session = { group_sessions = [] } in
-  let session_bytes: dy_bytes = serialize group_manager_state session in
-  parse_serialize_inv_lemma #dy_bytes group_manager_state session;
-  new_session pr group_manager_label group_manager_invariant p si 0 session_bytes;
-  si
-#pop-options
-
-val set_group_manager:
-  pr:preds -> p:principal -> si:nat ->
-  st:group_manager_state ->
-  LCrypto unit pr
-  (requires fun t0 -> group_manager_state_invariant pr.global_usage (trace_len t0) st /\ has_group_manager_invariant pr)
-  (ensures fun t0 r t1 -> trace_len t1 == trace_len t0 + 1)
-let set_group_manager pr p si st =
-  let st_bytes: dy_bytes = serialize group_manager_state st in
-  parse_serialize_inv_lemma #dy_bytes group_manager_state st;
-  update_session pr group_manager_label group_manager_invariant p si 0 st_bytes
-
-val get_group_manager:
-  pr:preds -> p:principal -> si:nat ->
-  LCrypto group_manager_state pr
-  (requires fun t0 ->  has_group_manager_invariant pr)
-  (ensures fun t0 st t1 ->
-    group_manager_state_invariant pr.global_usage (trace_len t0) st /\
-    t1 == t0
-  )
-let get_group_manager pr p si =
-  let (_, st_bytes) = get_session pr group_manager_label group_manager_invariant p si in
-  Some?.v (parse group_manager_state st_bytes)
-
-#push-options "--fuel 1"
-val add_new_group_sessions:
-  pr:preds -> p:principal -> si:nat ->
-  x:group_manager_state_elem ->
-  LCrypto unit pr
-  (requires fun t0 ->
-    is_publishable pr.global_usage (trace_len t0) x.group_id /\
-    has_group_manager_invariant pr
-  )
-  (ensures fun t0 () t1 -> trace_len t1 == trace_len t0 + 1)
-let add_new_group_sessions pr p si x =
-  let st = get_group_manager pr p si in
-  let new_st = { group_sessions = x::st.group_sessions } in
-  set_group_manager pr p si new_st
-#pop-options
-
-#push-options "--fuel 1 --ifuel 1"
-val find_group_sessions_aux: group_id:mls_bytes dy_bytes -> l:list group_manager_state_elem -> Pure (option group_manager_state_elem)
-  (requires True)
-  (ensures fun res ->
-    match res with
-    | None -> True
-    | Some x -> x.group_id == group_id /\ List.Tot.memP x l
-  )
-let rec find_group_sessions_aux group_id l =
-  match l with
-  | [] -> None
-  | h::t ->
-    if h.group_id = group_id then
-      Some h
-    else
-      match find_group_sessions_aux group_id t with
-      | Some res -> Some res
-      | None -> None
-#pop-options
-
-val find_group_sessions:
-  pr:preds -> p:principal -> si:nat ->
-  group_id:mls_bytes dy_bytes ->
-  LCrypto group_manager_state_elem pr
-  (requires fun t0 ->
-    has_group_manager_invariant pr
-  )
-  (ensures fun t0 x t1 ->
-    is_publishable pr.global_usage (trace_len t0) x.group_id /\
-    t1 == t0
-  )
-let find_group_sessions pr p si group_id =
-  let st = get_group_manager pr p si in
-  match find_group_sessions_aux group_id st.group_sessions with
-  | None -> error "find_group_sessions no sessions found!"
-  | Some x -> (
-    let now = global_timestamp () in
-    group_manager_state_invariant_eq pr.global_usage now st;
-    x
-  )
+let initialize_group_manager = initialize_map group_manager_types group_manager_pred group_manager_label
+let add_new_group_sessions = add_key_value group_manager_types group_manager_pred group_manager_label
+let find_group_sessions = find_value group_manager_types group_manager_pred group_manager_label
